2.2

Chapter1/chapter1.dfy
@@ -1,44 +1,134 @@
-// change
-
-method Triple (x: int) returns (r: int)
-  ensures r == 3 * x
-  {
-    var y := 2 * x;
-    r := x + y;
-  }
-method Triple2 (x: int) returns (r: int){
-  if x == 0 {
-    r := 0;
-  }
-  else {
-    var y := 2 * x;
-    r := x + y;
-  }
-  assert r == 3 * x;
-}
-method Triple3 (x: int) returns (r: int) {
-  if {
-    case x < 18 =>
-      var a, b := 2 * x, 4 * x;
-      r := (a + b ) / 2;
-    case 0 <= x =>
+// Triple
+  method Triple (x: int) returns (r: int)
+    ensures r == 3 * x
+    {
       var y := 2 * x;
       r := x + y;
+    }
+  method Triple2 (x: int) returns (r: int){
+    if x == 0 {
+      r := 0;
+    }
+    else {
+      var y := 2 * x;
+      r := x + y;
+    }
+    assert r == 3 * x;
   }
-  assert r == 3 * x;
-}
-method Triple4 (x: int) returns (r: int)
-  requires x == 0
-  ensures r == 3 * x
-  {
-    var y := x / 2;
-    r := 6 * y;
+  method Triple3 (x: int) returns (r: int) {
+    if {
+      case x < 18 =>
+        var a, b := 2 * x, 4 * x;
+        r := (a + b ) / 2;
+      case 0 <= x =>
+        var y := 2 * x;
+        r := x + y;
+    }
+    assert r == 3 * x;
+  }
+  method Triple4 (x: int) returns (r: int)
+    requires x == 0
+    ensures r == 3 * x
+    {
+      var y := x / 2;
+      r := 6 * y;
+    }
+
+  method Caller () {
+    var t := Triple(18);
+    assert t < 100;
   }
 
-method Caller () {
-  var t := Triple(18);
-  assert t < 100;
+// Max Sum
+  method Min (x: int, y: int) returns (m: int)
+    ensures m <= x && m <= y
+    ensures m == x || m == y
+    {
+      if x < y {
+        m := x;
+      } else if y < x {
+        m := y;
+      }
+      else{
+        m := x;
+      }
+    }
+
+  method MaxSum(x: int, y: int) returns (s: int, m: int)
+    ensures m >= x && m >= y && (m == x || m == y)
+    ensures s == x + y
+    {
+      if x >= y {
+        m := x;
+      } else {
+        m := y;
+      }
+      s := x + y;
+    }
+
+  method MSCaller(){
+    var sum, max := MaxSum(1928, 1);
+    assert sum == 1929;
+    assert max == 1928;
+  }
+  method ReconstructFromMaxSum(s: int, m: int) returns (x: int, y: int)
+    requires s <= 2 * m
+    ensures s == x + y
+    ensures (m == x || m == y) && m >= x && m >= y
+    {
+      x := m;
+      y := s - x;
+    }
+  method TestMaxSum(x: int, y: int){
+    var s, m := MaxSum(x, y);
+    var x_, y_ := ReconstructFromMaxSum(s, m);
+    assert (x_ == x && y_ == y) || (x_ == y && y_ == x);
+  }
+
+// Average
+  function Average(a: int, b: int): int{
+    (a + b) / 2 
+  }
+  method Triple'(x: int) returns (r: int)
+    ensures Average(r, 3 * x) == 3 * x
+    ensures Average(r + 1, 3 * x) == 3 * x
+    // {
+    //   //r equals someting that averages to 3*x with 3*x, but is not 3 * x
+    //   //r := 3 * x + 1;
+    //   r := 3 * x + 1;
+    // }
+  method CheckTriple'(x: int){
+    var r1 := Triple(x);
+    var r2 := Triple'(x);
+    assert r1 == r2;
+  }
+
+  function Average''(a: int, b: int): int{
+    (a + b) / 2 
+  }
+  ghost method Triple''(x: int) returns (r: int)
+    ensures r == 3 * x
+    {
+      ghost var bunny := 100;
+      r := Average''(2 * x, 4 * x);
+    }
+
+// 1.11
+function F(): int{
+  29
 }
+
+method M() returns (r: int){
+  r := 29;
+}
+
+method Caller'() {
+  var a := F();
+  var b := M();
+  assert a == 29;
+  assert b == 29;
+}
+
 
 method Main()
 {
