Chapter2/chapter2.dfy
@@ -1,0 +1,56 @@
+method MyMethod(x: int) returns (y: int)
+  requires 10 <= x
+  ensures 25 <= y
+{
+  var a, b;
+  a := x + 3;
+  if x < 20 {
+    b := 32 - x;
+  }
+  else {
+    b := 16;
+  }
+  y := a + b;
+}
+
+// Exercise 2.0
+method MyMethod_two_point_zero(x: int) returns (y: int)
+  requires x == 18
+  ensures 25 <= y
+{
+  var a, b;
+  a := x + 3;
+  if x < 20 {
+    b := 32 - x;
+  }
+  else {
+    b := 16;
+  }
+  y := a + b;
+
+  // program state at (9)
+  assert a == 21;
+  assert b == 14;
+  assert y == 35;
+
+  // program state (10)
+  // y == 35;
+}
+
+// Exercise 2.1
+/* Prove 10 <= x && a == x + 3 && b == 12 && y == a + b ==> 25 <= y
+  is a valid formula, aka a formula that evaluates to true for any values
+  10 <= a - 3 ==> 13 <= a
+  13 + 12 <= a + b == y
+  25 <= y
+*/
+
+// Exercise 2.2
+/* Prove 10 <= x ==> 25 <= x + 3 + 12
+  25 <= x + 15 == x + 3 + 12
+*/
+     
+
+method Main() {
+  print "Hello, Dafny!";
+}
